src/Quarantine.fst
@@ -4,7 +4,11 @@ let quarantine_slab arr = if enable_quarantine_trap then trap_array arr else A.v
 
 let mmap_trap_quarantine arr len =
   if enable_quarantine_trap then (
-    mmap_trap arr len;
+    if enable_quarantine_strict_trap then (
+      mmap_strict_trap arr len
+    ) else (
+      mmap_trap arr len
+    );
     change_equal_slprop (trap_array arr) (quarantine_slab arr)
   ) else (
     noop ();
